Base Grep naive

Part 2 - Dafny/grep-naive/grep.dfy
@@ -7,8 +7,125 @@
 
 include "Io.dfy"
 
+predicate inRange(i: int, len: int, j: int, len2: int) {
+  0 <= i < len && 0 <= j < len2
+}
+
+method Grep(word: array<byte>, query: array<char>) returns (found: string, pos: int)
+requires word.Length > 0
+requires query.Length > 0
+{
+  var i, j := 0, 0;
+  found := "";
+
+  while (i < word.Length && j < query.Length) 
+  invariant i <= word.Length
+  invariant j <= query.Length
+  invariant j <= i
+  // j > 0 && j < query.Length && i >= 0 && i < word.Length && w
+  // decreases if inRange(i, word.Length, j, query.Length) && word[i] == query[j] then query.Length - j else if inRange(i, word.Length, j, query.Length) &&  word[i] != query[j] && j > 0 then i - word.Length else word.Length - i
+  {
+    if word[i] as char == query[j] {
+      if j == 0 {found := "YES";  pos := i;    }
+      j := j + 1;
+    } else if j > 0 {
+      var p_j := j;
+      j := 0;
+      if p_j > 0 && word[i] as char == query[j] {
+        found := "YES"; //+ i as char;
+        pos := i;
+        j := j + 1;
+      }
+      //i := i - 1;
+    } 
+    
+    i := i + 1;
+  }
+  if found == "" {
+    found := "NO";
+    pos := 0;
+  }
+}
+
 method {:main} Main(ghost env:HostEnvironment?)
   requires env != null && env.Valid() && env.ok.ok();
+    modifies env.ok
+  modifies env.files
 {
-  print "TODO!\n";  
+  var ncmd := HostConstants.NumCommandLineArgs(env);
+
+    if ncmd != 3 {
+      if ncmd >= 1 {
+        print ncmd - 1; print " files supplied.\n";
+      }
+      print "Command requires src file and dst file... Example: ./reverse.exe Source Dest\n";
+      return;
+    }
+
+    var srcFile := HostConstants.GetCommandLineArg(1, env);
+    var query := HostConstants.GetCommandLineArg(2, env);
+
+    var ok;
+
+    ok := FileStream.FileExists(srcFile, env);
+
+    if !ok {
+      print "In file '"; print srcFile; print "'doesn't exist";
+      return;
+    }
+
+    var len;
+
+    ok, len := FileStream.FileLength(srcFile, env);
+
+    if !ok {
+      print "Couldn't stat file '"; print srcFile; print "' length";
+      return;
+    }
+    
+    var fs;
+
+    ok, fs := FileStream.Open(srcFile, env);
+    
+    if !ok {
+      print "Problems opening file "; print srcFile; print "\n";
+      return;
+    }
+
+    var buffer := new byte[len];
+    ok := fs.Read(0, buffer, 0, len);
+
+    if !ok {
+      print "Problems reading in file'"; print srcFile; print "'\n";
+      return;
+    }
+
+    var i := buffer.Length;
+
+    ok := fs.Close();
+
+    if !ok {
+      print "Problems closing in file '"; print srcFile; print "'\n";
+      return;
+    }
+
+    if buffer.Length == 0 {
+      print "File is empty, exiting.";
+      return;
+    }
+    if query.Length == 0 {
+      print "Empty query, exiting.";
+      return;
+    }
+
+    
+    var found, pos:= Grep(buffer, query);
+    
+    if found == "YES"{
+     print found,", ", pos;
+    }
+    else {
+      print found;
+    }
+
 }
